Allow expansion of Forall_parse_of

src/Parsers/ContextFreeGrammarProperties.v
@@ -6,33 +6,75 @@ Set Implicit Arguments.
 Delimit Scope string_like_scope with string_like.
 
 Section cfg.
-  Context CharType (String : string_like CharType) (G : grammar CharType)
-          (P : String -> String.string -> Type).
+  Context CharType (String : string_like CharType) (G : grammar CharType).
 
-  Fixpoint Forall_parse_of {str pats} (p : parse_of String G str pats)
-    := match p with
-         | ParseHead str pat pats p'
-           => Forall_parse_of_production p'
-         | ParseTail _ _ _ p'
-           => Forall_parse_of p'
-       end
-  with Forall_parse_of_production {str pat} (p : parse_of_production String G str pat)
-       := let Forall_parse_of_item {str it} (p : parse_of_item String G str it)
-              := match p return Type with
-                   | ParseTerminal x => unit
-                   | ParseNonTerminal name str p'
-                     => (P str name * Forall_parse_of p')%type
-                 end in
-          match p return Type with
-            | ParseProductionNil => unit
-            | ParseProductionCons str pat strs pats p' p''
-              => (Forall_parse_of_item p' * Forall_parse_of_production p'')%type
-          end.
+  Section definitions.
+    Context (P : String -> String.string -> Type).
 
-  Definition Forall_parse_of_item {str it} (p : parse_of_item String G str it)
-    := match p return Type with
-         | ParseTerminal x => unit
-         | ParseNonTerminal name str p'
-           => (P str name * Forall_parse_of p')%type
-       end.
+    Definition Forall_parse_of_item'
+               (Forall_parse_of : forall {str pats} (p : parse_of String G str pats), Type)
+               {str it} (p : parse_of_item String G str it)
+      := match p return Type with
+           | ParseTerminal x => unit
+           | ParseNonTerminal name str p'
+             => (P str name * Forall_parse_of p')%type
+         end.
+
+    Fixpoint Forall_parse_of {str pats} (p : parse_of String G str pats)
+      := match p with
+           | ParseHead str pat pats p'
+             => Forall_parse_of_production p'
+           | ParseTail _ _ _ p'
+             => Forall_parse_of p'
+         end
+    with Forall_parse_of_production {str pat} (p : parse_of_production String G str pat)
+         := match p return Type with
+              | ParseProductionNil => unit
+              | ParseProductionCons str pat strs pats p' p''
+                => (Forall_parse_of_item' (@Forall_parse_of) p' * Forall_parse_of_production p'')%type
+            end.
+
+    Definition Forall_parse_of_item {str it} (p : parse_of_item String G str it)
+      := @Forall_parse_of_item' (@Forall_parse_of) str it p.
+  End definitions.
+
+  Section expand.
+    Context (P P' : String -> String.string -> Type)
+            (f : forall str n, P str n -> P' str n).
+
+    Definition expand_forall_parse_of_item'
+               {Forall_parse_of : forall P {str pats} (p : parse_of String G str pats), Type}
+               (expand : forall {str pats p}, @Forall_parse_of P str pats p -> @Forall_parse_of P' str pats p)
+               {str it p}
+    : @Forall_parse_of_item' P (@Forall_parse_of P) str it p
+      -> @Forall_parse_of_item' P' (@Forall_parse_of P') str it p.
+    Proof.
+      destruct p; simpl.
+      { exact (fun x => x). }
+      { intro ab.
+        exact (f (fst ab), expand _ _ _ (snd ab)). }
+    Defined.
+
+    Global Arguments expand_forall_parse_of_item' : simpl never.
+
+    Fixpoint expand_forall_parse_of {str pats} (p : parse_of String G str pats)
+    : Forall_parse_of P p -> Forall_parse_of P' p
+      := match p return Forall_parse_of P p -> Forall_parse_of P' p with
+           | ParseHead str pat pats p'
+             => expand_forall_parse_of_production p'
+           | ParseTail _ _ _ p'
+             => expand_forall_parse_of p'
+         end
+    with expand_forall_parse_of_production {str pat} (p : parse_of_production String G str pat)
+         : Forall_parse_of_production P p -> Forall_parse_of_production P' p
+         := match p return Forall_parse_of_production P p -> Forall_parse_of_production P' p with
+              | ParseProductionNil => fun x => x
+              | ParseProductionCons str pat strs pats p' p''
+                => fun ab => (expand_forall_parse_of_item' (@expand_forall_parse_of) (fst ab),
+                              expand_forall_parse_of_production p'' (snd ab))
+            end.
+
+    Definition expand_forall_parse_of_item {str it} (p : parse_of_item String G str it)
+      := @expand_forall_parse_of_item' _ (@expand_forall_parse_of) str it p.
+  End expand.
 End cfg.
